\section{Appendix A - Derivation of activation functions} \label{sec:appendixa}

\subsection{Sigmoid} \label{sec:sigmoid_der}
If we differentiate the sigmoid function 
\begin{equation}
f(x)=\frac{1}{1+\exp(-x)}
\end{equation}
from equation (\ref{eq:sigmoid}), and we will get
\begin{equation}
f'(x)=f(1-f)
\end{equation}

\textbf{PROOF:}
\begin{align*}
f'(x) &= -1\cdot(1+\exp(-x))^{-2}\cdot -1\cdot\exp(-x)\\
&=\frac{\exp(-x)}{(1+\exp(-x))^{2}}\\
&=\frac{1+\exp(-x)-1}{(1+\exp(-x))^{2}}\\
&=\frac{1+\exp(-x)}{(1+\exp(-x))^{2}} - \frac{1}{(1+\exp(-x))^{2}}\\
&=\frac{1}{1+\exp(-x)} - \frac{1}{(1+\exp(-x))^{2}}\\
&=\frac{1}{1+\exp(-x)}\bigg(1 - \frac{1}{1+\exp(-x)}\bigg)\\
&=f(1-f)
\end{align*}

\subsection{Cross-entropy}